theories/ITree/Logic/Lemmas.v
@@ -10,6 +10,7 @@ From ExtLib Require Import
   Data.Monads.StateMonad.
 
 From CTree Require Import
+  Events.Core
   ITree.Core
   ITree.Equ
   ITree.Logic.Trans
@@ -26,68 +27,210 @@ Local Open Scope itree_scope.
 
 (*| CTL logic lemmas on c/itrees |*)
 Section CtlITrees.
-  Context {W X: Type}.
-  Notation itreeW W X := (itree (writerE W) X).
+  Context {E: Type} {HE: Encode E}.
 
-  Lemma ctl_af_star: forall (t: itreeW W X * option W) φ,
-      <( t |= AF φ )> <-> ( exists t', t ↦* t' /\ <( t' |= φ )>).
+  Lemma ctl_af_star{X}: forall (t: itree E X * World E) φ,
+      <( t |= AF φ )> -> exists t', t ↦* t' /\ <( t' |= φ )>.
   Proof.
-    cbn; split; intros.
+    cbn; intros.
     dependent induction H.
     + exists m; split.
-      * exists 0%nat; reflexivity.
+      * exists 0%nat; cbn; auto. 
       * assumption.
-    + destruct H1 as [(? & ?) ?].
-      destruct (H2 _ H1) as [[? ?] (? & ?)].
-      destruct H3 as (n & ?).
-      exists (k, w); split; auto.
+    + destruct H1 as [(te & we & TRe) ?].
+      destruct (H1 _ TRe) as [[t' w'] ((n & TRn) & ?)].
+      exists (t', w'); split; auto.
       exists (S n).
-      cbn; unfold hrel_dot.
-      exists x; auto.
-    + destruct H as (t' & [n ?] & Hφ).
-      generalize dependent t.
-      revert t' Hφ.
-      induction n; intros; cbn in H.
-      * apply ctl_af_ax.
-        left.
-        now rewrite H.
-      * apply ctl_af_ax.
-        right.
-        apply ctl_ax.
-        destruct H as [t0 TR0 TRn].
-        split; [now exists t0|].
-        intros.
-        pose proof (trans_det (W:=W) (X:=X) _ _ _ TR0 H).
-        eapply IHn with t'; auto.
-        now rewrite <- H0.
+      cbn.
+      exists (te, we); destruct m as (t, w); split; auto.
   Qed.
 
-  Lemma ctl_star_ef: forall (t:  itreeW X * W) φ,
-      (exists t', t ↦* t' /\ <( t' |= φ )>) <-> <( t |= EF φ )>.
+  Lemma can_step_bind_iff{X Y}: forall (t: itree E Y) (k: Y -> itree E X) w,
+      can_step (x <- t ;; k x, w) <->        
+        (exists t' w', (t, w) ↦ (t', w') /\ not_done w')
+        \/ (exists y w', (t, w) ↦ (Itree.stuck, w')
+                   /\ return_with y w'
+                   /\ can_step (k y, w)).
   Proof.
-    split.
-    - intros (t' & [n Iter] & Hφ).
-      revert Hφ.
-      revert t t' φ Iter.
-      induction n; intros; cbn in Iter.
-      + rewrite Iter.
-        now rewrite ctl_ef_ex; left.
-      + red in Iter.
-        destruct (Iter) as [t0 Htr Htt]; clear Iter.
-        specialize (IHn _ _ _ Htt Hφ).
-        rewrite ctl_ef_ex; right; cbn.
-        exists t0; split; auto.
-    - intro H.
-      induction H.
-      + exists m; split; auto.
-        exists 0; cbn; reflexivity.
-      + destruct H1 as (m' & TR & m'' & TRn & ?).
-        exists m''; split; [|auto].
-        destruct TRn as (n & ?).
-        exists (S n); cbn; unfold hrel_dot.
-        exists m'; auto.
+    unfold can_step; split.
+    - intros (k' & w' & TR).
+      apply ktrans_bind_inv in TR
+          as [(t' & TR' & Hd & ?) | (y & w_ & ? & Hd & ?)].
+      + left; exists t', w'; auto.
+      + right; inv Hd.
+        * exists y, (Done y); eauto with ctl.
+        * exists y, (Finish e v y); eauto with ctl.
+    - intros * [(t' & w' & TR & Hd) | (y & w' & TR & Hd & k_ & w_ & TR_)]; cbn in TR; dependent induction TR.       
+      + observe_equ x0; cbn.
+        setoid_rewrite Eqt.
+        setoid_rewrite bind_vis.
+        exists (x <- k0 v ;; k x), (Obs e v); now apply KtransObs.
+      + observe_equ x0; cbn in *.
+        setoid_rewrite Eqt.
+        setoid_rewrite bind_tau.
+        destruct (IHTR t0 k w _ _ eq_refl eq_refl Hd)
+          as (t_ & w_ & TR_).
+        exists t_, w_; apply KtransTau; auto.
+      + inv Hd.
+      + inv Hd.
+      + inv Hd.
+      + observe_equ x0; cbn in *.
+        setoid_rewrite Eqt.
+        setoid_rewrite bind_tau.
+        cbn.
+        assert (Heq: (observe t', w') = (TauF Itree.stuck, w')) by now rewrite x.
+        destruct (IHTR t0 k w _ eq_refl Heq Hd k_ w_ TR_)
+          as (k' & wk' & TRk').        
+        exists k', wk'; apply KtransTau; auto.
+      + observe_equ x1; dependent destruction Hd; cbn in *.
+        setoid_rewrite Eqt.
+        setoid_rewrite bind_ret_l.
+        exists k_, w_; auto.
+      + observe_equ x1; dependent destruction Hd; cbn in *.
+        setoid_rewrite Eqt.
+        setoid_rewrite bind_ret_l.
+        exists k_, w_; auto.
+  Qed.
+  Hint Resolve can_step_bind_iff: ctl.
+
+  Lemma can_step_bind_l{X Y}: forall (t t': itree E Y) (k: Y -> itree E X) w w',
+      (t, w) ↦ (t', w') ->
+      not_done w' ->
+      can_step (x <- t ;; k x, w).
+  Proof.
+    intros.
+    eapply can_step_bind_iff.
+    left; eauto.
+  Qed.
+  Hint Resolve can_step_bind_l: ctl.
+
+  Lemma ctl_stuck_obs_af{X}: forall (x: X) φ w,
+      return_with x w ->
+      ~ <( {(Itree.stuck: itree E X, w)} |= AF obs φ )>.
+  Proof.
+    intros * Hret Hcontra.
+    inv Hcontra.
+    - rewrite ctl_obs in H.
+      destruct H as (? & ? & ? & ?); cbn in *; subst.
+      inv Hret.
+    - destruct H0 as ((? & ? & ?) & ?).
+      now apply ktrans_stuck in H0.
   Qed.
 
+  Lemma ctl_obs_af_inv{X}: forall (t: itree E X) φ w,
+      <( {(t, w)} |= AF obs φ )> ->
+      not_done w.  
+  Proof.
+    intros * Haf.
+    next in Haf; destruct Haf; cbn in H.
+    - destruct H as (e & v & -> & ?).
+      constructor.
+    - destruct H. 
+      destruct H as (t' & w' & TR).
+      now eapply ktrans_not_done with t t' w'.
+  Qed.
+  Hint Resolve ctl_obs_af_inv: ctl.
+
+  Opaque entailsF.
+  Theorem ctl_bind_af_l{X Y}: forall (t: itree E Y) (k: Y -> itree E X) φ w,
+      <( {(t, w)} |= AF obs φ )> ->
+      <( {(x <- t ;; k x, w)} |= AF obs φ )>.
+  Proof.
+    intros * Haf.
+    remember (t, w) as m.
+    replace t with (fst m) by now subst.
+    replace w with (snd m) by now subst.
+    clear Heqm t w.
+    revert X k.
+    induction Haf; intros; destruct m as [t w]; subst; cbn in *.
+    - (* MatchA *)
+      next; left; cbn.
+      destruct H as (e_ & x_ & ? & ?); subst.
+      rewrite ctl_obs; eauto.
+    - (* StepA *)
+      destruct H0, H1; clear H H0.
+      destruct H1 as (te & we & TR); cbn in *.
+      dependent destruction TR.
+      + next; right; next; split. 
+        * apply can_step_bind_l with t0 (Obs e v); cbn. 
+          -- rewrite <- x0.
+             now apply KtransObs.
+          -- constructor.
+        * intros [k' w'] TR'.
+          apply ktrans_bind_inv in TR'
+              as [(t' & TR' & Hd & ?) | (y & w_ & TRt' & Hr & TRk)].
+          -- rewrite H1.
+             specialize (H3 (t', w') TR').
+             apply H3.
+          -- specialize (H2 (Itree.stuck, w_) TRt').
+             Transparent entailsF.
+             apply ctl_stuck_obs_af with (x:=y) in H2; intuition.             
+      + observe_equ x0.
+        rewrite Eqt.
+        assert (TRtau: trans_ (observe t, w) (observe t', we)).
+        { rewrite x0; now apply KtransTau. }        
+        next; right; next; split. 
+        * eapply can_step_bind_l; cbn.
+          apply KtransTau; eauto.
+          specialize (H3 (t', we) TRtau _ k); cbn in H3.        
+          now apply ctl_obs_af_inv in H3.
+        * intros [k' w'] TR'.
+          apply ktrans_bind_inv in TR'
+              as [(t_ & TR_ & Hd & ?) | (y & w_ & TRt' & Hd & TRk) ].
+          -- rewrite H.
+             specialize (H3 (t_, w')); cbn in H2.
+             rewrite ktrans_tau in TR_.
+             apply H3.
+             rewrite x0.
+             now apply ktrans_tau.
+          -- cbn in TRt'.
+             rewrite <- x0 in TRt'.
+             specialize (H2 (Itree.stuck, w_) TRt'); cbn in H2.             
+             Transparent entailsF.
+             eapply ctl_stuck_obs_af with (x:=y) in H2; intuition. 
+      + assert (TRt: trans_ (observe t, Pure) (observe Itree.stuck, Done x0)).
+        { rewrite <- x1; apply KtransDone; reflexivity. }.
+        specialize (H3 (Itree.stuck, Done x0) TRt _ k); cbn in H3.
+        apply ctl_obs_af_inv in H3; inv H3.
+      + assert (TRt: trans_ (observe t, Obs e v) (observe Itree.stuck, Finish e v x0)).
+        { rewrite <- x1; apply KtransFinish; reflexivity. }.
+        specialize (H3 (Itree.stuck, Finish e v x0) TRt _ k).
+        apply ctl_obs_af_inv in H3; inv H3.
+  Qed.
+
+  Lemma can_step_bind_r{X Y} {HP: Productive E}:
+    forall (t: itree E Y) (k: Y -> itree E X) w (r: Y),      
+      <( {(t, w)} |= AF return r )> ->
+      can_step (k r, w) ->
+      can_step (x <- t ;; k x, w).
+  Proof.    
+    intros.
+    apply ctl_return_af_inv in H as [H|H].
+    - inv H. (* (kr, w) can step, so w != done *)
+      + inv H0; destruct H; inv H; inv H5.
+      + inv H0; destruct H; inv H; inv H5.
+    - revert w k H0.
+      remember (observe t) as T.
+      generalize dependent t.
+      generalize dependent X.            
+      induction H; intros; observe_equ HeqT; rewrite Eqt, ?bind_ret_l.
+      + exact H0.
+      + rewrite bind_br.
+        apply can_step_br; destruct b.
+        * destruct H1 as (? & ? & ?).
+          eapply ktrans_not_done; eauto.
+        * exists (Fin.F1).
+          eapply H0; try reflexivity; auto.
+      + rewrite bind_vis.
+        apply can_step_vis.
+        * (* Indeed, [x <- Vis (e: void) ;; k x]
+             does not step, ughhh *)
+          apply HP.
+        * destruct H1 as (? & ? & ?).
+          eapply ktrans_not_done; eauto.
+  Qed.
+  Hint Resolve can_step_bind_r: ctl.
+  
   Lemma iter_ctl_af: forall (t: X -> itreeW X) (σ: W) (i : X) (φ: W -> Prop),
       <( {(t i, σ)} |= AF done φ )> ->
       <( {(forever t i, σ)} |= AG AF now φ )>.
