theories/Logic/Semantics.v
@@ -200,7 +200,9 @@ Module CtlNotations.
 
   (* Temporal syntax: base *)
   Notation "'now' p" := (CBase p)
-                           (in custom ctl at level 74): ctl_scope.
+                          (in custom ctl at level 74): ctl_scope.
+  Notation "'return' r" := (CBase (return_with r))
+                             (in custom ctl at level 74): ctl_scope.
   Notation "'pure'" := (CBase (fun w => w = Pure))
                          (in custom ctl at level 74): ctl_scope.
   Notation "'obs' p" := (CBase (fun o => exists e x, o = Obs e x /\ p e x))
